sticker/TPP.v
@@ -1,0 +1,29 @@
+From mathcomp Require Import all_ssreflect.
+
+Fixpoint Rewrite{t:Type}(n:nat)(x:t)(s:seq t):seq t:=
+match n, s with
+|0, h::s' => x::s'
+|S n', h::s' => h::Rewrite n' x s'
+|_, nil => nil
+end.
+Compute Rewrite 2 5 [::1;2;3;4;5].
+Definition Swap(n m:nat)(s:seq nat):seq nat :=
+Rewrite n(nth 0 s m)(Rewrite m(nth 0 s n)s).
+Compute Swap 2 5 [::0;1;2;3;4;5;6].
+(*indexは0から*)
+Notation "( x | y ) z":=(Swap x y z)(at level 41,right associativity) .
+
+Fixpoint Cycle(x s:seq nat): seq nat :=
+match x with
+|a::x' =>
+  match x' with
+  |nil => s
+  |b::_ => Swap a b(Cycle x' s)
+  end
+|nil => nil
+end.
+
+Compute Cycle[::1;4;3][::5;9;1;3;7].
+Compute Cycle[::0;1;3;4;2][::0;1;2;3;4].
+Eval simpl in Cycle[::0;1;3;4;2].
+Theorem minSwapCycle(x:seq nat)
